Ajustement des définitions du zéro-copie

src/CoqNom/examples/example3.v
@@ -7,9 +7,11 @@ Import N.
 From Formalisation Require Export Span.
 From FreeMonad Require Import FreeMonad.
 From SepLogic Require Import SepSet.
-From Formalisation Require Import IsFresh Inject.
+From Formalisation Require Import IsFresh Inject ZeroCopy.
 From Classes Require Import Foldable.
 From Examples Require Import example2.
+
+Require Import Coq.Program.Equality.
 
 Open Scope N_scope.
 
@@ -67,7 +69,7 @@ Proof.
 Qed.
 
 
-Notation "{{ P }} m {{ v ; Q }}" := (P ⊢ wp m (fun v => Q))
+Notation "{{ P }} m {{ v ; Q }}" := (⊢ P -∗ wp m (fun v => Q))
                                       (at level 20,
                                         format "'[hv' {{  P  }}  '/  ' m  '/'  {{  v ;  Q  }} ']'").
 
@@ -303,4 +305,81 @@ Proof.
   injection H0. intro. subst. eapply soundness_pure.
   iIntros "HA". iApply (soundness _ d emp (fun v => ⌜ Q v ⌝)); eauto.
   iSplitR; auto. simpl. iApply big_op_ctx. eauto.
+Qed.
+
+Lemma Fresh_ZC_aux `{Foldable M}: forall e s n s_res,
+    {{ injectSL n (pos s) }} e {{ res; <absorb> all_disjointMSL res }} ->
+    forall (data : data) (res : M span),
+      n <= pos s ->
+      eval e data s = Some (res, s_res) ->
+      forall v, v ∈ M_to_list res ->
+           set_span v ⊆ inject n (pos s + len s).
+Proof.
+  revert M H. fix IH 3. intros M H e.
+  dependent destruction e; intros; simpl in *. revert H1 H2. intros LE H1.
+  - inversion H1. subst. clear H1.
+    revert H0. MonPred.unseal. unfold monpred.monPred_wand_def. simpl.
+    unfold monpred.monPred_upclosed. simpl. intro. destruct H0. simpl in *.
+    edestruct (monPred_in_entails tt). clear monPred_in_entails.
+    instantiate (1 := ∅). MonPred.unseal.
+    split. split. inversion_star h P. clear H0.
+    red in P1. destruct P1. inversion H1. subst. clear H1. clear P2.
+    rewrite union_empty_r_L in P. clear monPred_in_entails. subst.
+    edestruct H0.
+    + eexists ∅, _. repeat split; auto. 2 : eapply disjoint_empty_l.
+      eapply SepSet.soundness. iIntros "HA". iApply big_op_ctx. iApply "HA".
+    + destruct H1 as [h [P3 [P1 [P2 P4]]]]. clear H0 P0 P3.
+      rewrite union_empty_l_L in P4.
+      transitivity (inject n (Span.pos s_res)).
+      2 : { eapply inject_mono_r. lia. }
+      rewrite P4. transitivity h. 2 : set_solver. clear P2 P4. unfold all_disjointMSL in P1.
+      eapply (all_disjointSL_incl _ _ H3 _ P1).
+  - destruct d; simpl in *.
+    + unfold set_span.
+      unfold bind, takeM in H2.
+      destruct (n0 <=? len s) eqn:?.
+      * pose (mono := H2). eapply eval_monotone in mono as [P0 P1]. simpl in *.
+        eapply N.leb_le in Heqb. assert (pos s + len s = pos s + n0 + (len s - n0)) by lia.
+        rewrite H4.
+        unfold set_span in IH.
+        eapply (IH _ _ _ {| pos := pos s + n0; len := len s - n0 |}); simpl in *; eauto.
+        2 : lia.
+        iIntros "HA". unfold injectSL. rewrite (inject_add n0 n (pos s)). 2 : lia.
+        iDestruct (big_sepS_union with "HA") as "[HA HB]". eapply inject_disjoint.
+        iDestruct (inject_IsFresh with "[HB]") as "HB"; eauto.
+        unfold injectSL. instantiate (1 := (mk_span (pos s) n0)). simpl. iApply "HB".
+        iApply (H0 with "HA HB").
+      * inversion H2.
+    + unfold bind, readM in H2.
+      destruct (n0 <? len s0) eqn:?.
+      destruct (lookup (pos s0 + n0) data0) eqn:?.
+      eapply IH; eauto.
+      iIntros "HA". iDestruct (H0 with "HA") as "HB". iApply "HB".
+      inversion H2. inversion H2.
+    + inversion H2.
+Qed.
+
+
+Lemma eval_ZC `{Foldable M}: forall e,
+    {{ emp }} e {{ res; <absorb> all_disjointMSL res }} ->
+    forall (data : data) (res : M span) s s_res,
+      eval e data s = Some (res, s_res) ->
+      Result_in res s.
+Proof.
+  unfold Result_in. intros. eapply Fresh_ZC_aux.
+   iIntros "HA". iApply H0.
+   iApply (injectSL_emp with "HA"). lia. lia. eauto. auto.
+Qed.
+
+Definition decode_zerocopy `{Foldable M} (e : Decodeur (M span)) := forall data res,
+      decode e data = Some res ->
+      Result_in res (mk_span 0 (length data)).
+
+Lemma decode_ZC `{Foldable M}: forall e,
+    {{ emp }} e {{ res; <absorb> all_disjointMSL res }} ->
+    decode_zerocopy e.
+Proof.
+  unfold decode_zerocopy, decode. intros.
+  destruct eval as [[v s_v]|] eqn:?; inversion H1. subst.
+  eapply eval_ZC; eauto.
 Qed.
