src/CoqNom/src/Formalisation/ZeroCopy/ZeroCopy.v
@@ -1,0 +1,29 @@
+From stdpp Require Import numbers countable.
+From Formalisation Require Import Span SizeNat Inject IsFresh.
+From Classes Require Import Foldable.
+Require Import Vector.
+From Equations Require Import Equations.
+Import disjoint.
+
+Section ZeroCopy.
+
+  Context {M : Type -> Type}.
+  Context {foldable : Foldable M}.
+
+  Open Scope N_scope.
+
+  Definition set_span (s : span) := inject (pos s) (pos s + len s).
+
+  Definition scope_in (s t : span) := set_span s ⊆ set_span t.
+
+  Definition Result_in (r : M span) (s : span):=
+    forall v, v ∈ M_to_list r -> scope_in v s.
+
+  Definition WeakZC (decode : span -> option (M span)) :=
+    forall s (res : M span),
+      decode s = Some res ->
+      Result_in res s.
+
+  Close Scope N_scope.
+
+End ZeroCopy.
